theories/iris/logrel/instr/typing/cast.v
@@ -1,4 +1,5 @@
 Require Import RichWasm.iris.logrel.instr.typing.common.
+Require Import RichWasm.iris.logrel.instr.typing.type_eq.
 
 Set Bullet Behavior "Strict Subproofs".
 Set Default Goal Selector "!".
@@ -23,6 +24,24 @@ Section cast.
     has_instruction_type_ok F ψ L ->
     run_codegen (compile_instr mr fe (ICast ψ)) wt wl = inr ((), wt', wl', es') ->
     ⊢ have_instr_type_sem rti sr mr M F L WT WL lmask es' ψ L.
-  Admitted.
+  Proof.
+    intros fe WT WL lmask ψ Heq Hok Hcg.
+    inv_cg_ret Hcg.
+    subst ψ WT WL wt' wl' es'.
+    clear Hretval.
+    clear_nils.
+    destruct Hok as [[Hmono1 Hmono2] _].
+    rewrite Forall_singleton in Hmono1.
+    rewrite Forall_singleton in Hmono2.
+    destruct Hmono1 as (ρ1 & Hrep1 & _).
+    destruct Hmono2 as (ρ2 & Hrep2 & _).
+    inversion Hrep1 as [F1 τ1 ρ1' ξ1 Hkind1]; subst F1 τ1 ρ1'.
+    inversion Hrep2 as [F2 τ2 ρ2' ξ2 Hkind2]; subst F2 τ2 ρ2'.
+    iApply sem_type_erased; first done.
+    iIntros (se os) "%Hse Hv".
+    rewrite !values_interp_one_eq !value_interp_eq -!type_interp_eq.
+    iEval (rewrite (type_interp_type_eq rti sr _ _ Heq F _ _ se (SAtoms os) Hkind1 Hkind2 Hse)) in "Hv".
+    done.
+  Qed.
 
 End cast.
