theories/iris/logrel/instr/typing/type_eq.v
@@ -1,0 +1,343 @@
+Require Import RichWasm.iris.logrel.instr.typing.common.
+Require Import RichWasm.iris.logrel.instr.kinding.
+
+Set Bullet Behavior "Strict Subproofs".
+Set Default Goal Selector "!".
+
+Section serialize.
+
+  Lemma has_arep_serialize_length ι o :
+    has_arep ι o ->
+    length (serialize_atom o) = arep_size ι.
+  Proof.
+    intros H.
+    destruct ι, o; cbn in *; done.
+  Qed.
+
+  Lemma has_areps_serialize_length ιs os :
+    Forall2 has_arep ιs os ->
+    length (flat_map serialize_atom os) = areps_size ιs.
+  Proof.
+    induction 1 as [|ι o ιs os Hao HF IH]; cbn; first done.
+    rewrite length_app IH (has_arep_serialize_length _ _ Hao).
+    done.
+  Qed.
+
+  Lemma flat_map_concat {A B} (f : A -> list B) (ls : list (list A)) :
+    flat_map f (concat ls) = concat (map (flat_map f) ls).
+  Proof.
+    induction ls as [|l ls IH]; cbn; first done.
+    rewrite flat_map_app IH.
+    done.
+  Qed.
+
+  Lemma ref_flag_atom_word_serialize (P : pointer -> Prop) o :
+    forall_ptr_atom P o ->
+    Forall (forall_ptr_word P) (serialize_atom o).
+  Proof.
+    intros H.
+    destruct o; cbn in *; repeat constructor; done.
+  Qed.
+
+  Lemma ref_flag_serialize ξ os :
+    ref_flag_atoms_interp ξ (SAtoms os) ->
+    ref_flag_words_interp ξ (SWords (flat_map serialize_atom os)).
+  Proof.
+    unfold ref_flag_atoms_interp, ref_flag_words_interp, forall_satoms, forall_swords.
+    induction 1 as [|o os Ho Hos IH]; cbn; first constructor.
+    apply Forall_app.
+    split; last done.
+    by apply ref_flag_atom_word_serialize.
+  Qed.
+
+End serialize.
+
+Section pure_kinds.
+  Context {E : Type}.
+  Context `{Env E}.
+  Variable env : E.
+
+  Lemma eval_size_RepS_ProdR ρs :
+    eval_size env (RepS (ProdR ρs)) = eval_size env (ProdS (map RepS ρs)).
+  Proof.
+    cbn.
+    unfold compose.
+    induction ρs as [|ρ ρs IH]; cbn; first done.
+    destruct (eval_rep env ρ) as [ιs|] eqn:Hρ; cbn; last done.
+    destruct (mapM (eval_rep env) ρs) as [ιss|] eqn:Hρs;
+      destruct (mapM (eval_size env) (map RepS ρs)) as [ns|] eqn:Hns;
+      cbn in IH |- *; try done.
+    injection IH as IH.
+    f_equal.
+    rewrite map_app.
+    change (foldr Init.Nat.add 0 ?l) with (list_sum l).
+    change (foldr Init.Nat.add 0 ?l) with (list_sum l) in IH.
+    rewrite list_sum_app.
+    lia.
+  Qed.
+
+  Lemma eval_kind_valtype_inv ρ ξ ρ' ξ' :
+    eval_kind env (VALTYPE ρ ξ) = eval_kind env (VALTYPE ρ' ξ') ->
+    eval_rep env ρ = eval_rep env ρ' /\
+    (forall ιs, eval_rep env ρ = Some ιs -> ξ = ξ').
+  Proof.
+    cbn.
+    destruct (eval_rep env ρ) as [ιs|] eqn:Hρ;
+      destruct (eval_rep env ρ') as [ιs'|] eqn:Hρ'; cbn;
+      intros Heq; simplify_eq; split; congruence.
+  Qed.
+
+  Lemma eval_kind_ser_prod_struct ρs ξs ρs' ξs' :
+    Forall2 (fun ρξ ρξ' : representation * ref_flag =>
+               eval_kind env (VALTYPE ρξ.1 ρξ.2) = eval_kind env (VALTYPE ρξ'.1 ρξ'.2))
+      (zip ρs ξs) (zip ρs' ξs') ->
+    length ρs = length ξs ->
+    length ρs' = length ξs' ->
+    length ρs = length ρs' ->
+    eval_kind env (MEMTYPE (RepS (ProdR ρs)) (ref_flag_lub ξs)) =
+    eval_kind env (MEMTYPE (ProdS (map RepS ρs')) (ref_flag_lub ξs')).
+  Proof.
+    revert ξs ρs' ξs'.
+    induction ρs as [|ρ ρs IH]; intros ξs ρs' ξs' HF2 Hlen1 Hlen2 Hlen3;
+      destruct ρs' as [|ρ' ρs']; try discriminate;
+      destruct ξs as [|ξ ξs]; try discriminate;
+      destruct ξs' as [|ξ' ξs']; try discriminate.
+    - done.
+    - cbn in HF2.
+      apply Forall2_cons_1 in HF2 as [Hhd HF2].
+      apply eval_kind_valtype_inv in Hhd as [Hrep Hflag].
+      injection Hlen1 as Hlen1.
+      injection Hlen2 as Hlen2.
+      injection Hlen3 as Hlen3.
+      specialize (IH ξs ρs' ξs' HF2 Hlen1 Hlen2 Hlen3).
+      cbn in IH |- *.
+      unfold compose in *.
+      cbn in Hrep, Hflag.
+      destruct (eval_rep env ρ) as [ιs|] eqn:Hρ; rewrite <- Hrep; cbn; last done.
+      specialize (Hflag ιs eq_refl); subst ξ'.
+      destruct (mapM (eval_rep env) ρs) as [ιss|] eqn:Hρs;
+        destruct (mapM (eval_size env) (map RepS ρs')) as [ns|] eqn:Hns;
+        cbn in IH |- *; try done; try discriminate.
+      injection IH as IHn IHflag.
+      unfold ref_flag_lub in IHflag.
+      f_equal.
+      f_equal; last congruence.
+      rewrite map_app.
+      change (foldr Init.Nat.add 0 ?l) with (list_sum l).
+      rewrite list_sum_app.
+      lia.
+Qed.
+
+  Lemma struct_fields_ser_inv F κs_ser τs' σs' ξs2 :
+    Forall3 (fun τ σ ξ => has_kind F τ (MEMTYPE σ ξ)) (zip_with SerT κs_ser τs') σs' ξs2 ->
+    length κs_ser = length τs' ->
+    exists ρs2,
+      σs' = map RepS ρs2 /\
+      κs_ser = map (fun ρξ : representation * ref_flag => MEMTYPE (RepS ρξ.1) ρξ.2)
+                 (zip ρs2 ξs2) /\
+      Forall3 (fun τ' ρ ξ => has_kind F τ' (VALTYPE ρ ξ)) τs' ρs2 ξs2.
+  Proof.
+    revert τs' σs' ξs2.
+    induction κs_ser as [|κ0 κs_ser IH]; intros τs' σs' ξs2 HF3 Hlen;
+      destruct τs' as [|τ' τs']; try discriminate.
+    - cbn in HF3.
+      inversion HF3; subst.
+      exists [].
+      repeat split; constructor.
+    - cbn in HF3.
+      injection Hlen as Hlen.
+      inversion HF3 as [|? σ0 ξ0 ? σs0 ξs0 Hhd HF3']; subst.
+      inversion Hhd; subst.
+      destruct (IH _ _ _ HF3' Hlen) as (ρs2 & -> & -> & HF3'').
+      eexists (_ :: ρs2).
+      repeat split.
+      by constructor.
+  Qed.
+
+  Lemma eval_kind_pairs_of_kinds F τs τs' ρs ξs ρs2 ξs2 :
+    Forall2 (fun τ τ' =>
+               forall F κ κ',
+                 has_kind F τ κ ->
+                 has_kind F τ' κ' ->
+                 eval_kind env κ = eval_kind env κ') τs τs' ->
+    Forall3 (fun τ ρ ξ => has_kind F τ (VALTYPE ρ ξ)) τs ρs ξs ->
+    Forall3 (fun τ' ρ ξ => has_kind F τ' (VALTYPE ρ ξ)) τs' ρs2 ξs2 ->
+    Forall2 (fun ρξ ρξ' : representation * ref_flag =>
+               eval_kind env (VALTYPE ρξ.1 ρξ.2) = eval_kind env (VALTYPE ρξ'.1 ρξ'.2))
+      (zip ρs ξs) (zip ρs2 ξs2).
+  Proof.
+    intros HF2.
+    revert ρs ξs ρs2 ξs2.
+    induction HF2 as [|τ τ' τs τs' Hhd HF2 IH]; intros ρs ξs ρs2 ξs2 HF3 HF3'.
+    - inversion HF3; subst.
+      inversion HF3'; subst.
+      constructor.
+    - inversion HF3; subst.
+      inversion HF3'; subst.
+      cbn [zip zip_with].
+      constructor; last by apply IH.
+      cbv beta; cbn [fst snd].
+      by eapply Hhd.
+  Qed.
+
+  Lemma type_eq_eval_kind_agree :
+    forall τ τ',
+      type_eq τ τ' ->
+      forall F κ κ',
+        has_kind F τ κ ->
+        has_kind F τ' κ' ->
+        eval_kind env κ = eval_kind env κ'.
+  Proof.
+    apply (type_eq_ind'
+             (fun τ τ' =>
+                forall F κ κ',
+                  has_kind F τ κ ->
+                  has_kind F τ' κ' ->
+                  eval_kind env κ = eval_kind env κ')).
+    - intros τ F κ κ' Hκ Hκ'.
+      by rewrite (has_kind_agree _ _ _ _ Hκ Hκ').
+    - intros κ0 τs τs' _ _ F κ κ' Hκ Hκ'; inversion Hκ; inversion Hκ'; subst; congruence.
+    - intros κ0 τs τs' _ _ F κ κ' Hκ Hκ'; inversion Hκ; inversion Hκ'; subst; congruence.
+    - intros κ0 τs τs' _ _ F κ κ' Hκ Hκ'; inversion Hκ; inversion Hκ'; subst; congruence.
+    - intros κ0 τs τs' _ _ F κ κ' Hκ Hκ'; inversion Hκ; inversion Hκ'; subst; congruence.
+    - intros κ0 μ β τ τ' _ _ F κ κ' Hκ Hκ'; inversion Hκ; inversion Hκ'; subst; congruence.
+    - intros κ0 τ τ' _ _ F κ κ' Hκ Hκ'; inversion Hκ; inversion Hκ'; subst; congruence.
+    - intros κ0 τ τ' _ _ F κ κ' Hκ Hκ'; inversion Hκ; inversion Hκ'; subst; congruence.
+    - intros κ0 τ τ' _ _ F κ κ' Hκ Hκ'; inversion Hκ; inversion Hκ'; subst; congruence.
+    - intros κ0 τ τ' _ _ F κ κ' Hκ Hκ'; inversion Hκ; inversion Hκ'; subst; congruence.
+    - intros κ0 τ τ' _ _ F κ κ' Hκ Hκ'; inversion Hκ; inversion Hκ'; subst; congruence.
+    - intros κ0 κτ τ τ' _ _ F κ κ' Hκ Hκ'; inversion Hκ; inversion Hκ'; subst; congruence.
+    - intros κ_ser κ_prod κ_struct κs_ser τs τs' Hlen Heq IH F κ κ' Hκ Hκ'.
+      inversion Hκ; subst.
+      match goal with Hp : has_kind _ (ProdT _ _) _ |- _ => rename Hp into Hprod end.
+      inversion Hprod; subst.
+      match goal with Hf : Forall3 _ τs _ _ |- _ => rename Hf into HF3 end.
+      inversion Hκ'; subst.
+      match goal with
+        Hf : Forall3 _ (zip_with SerT _ _) _ _ |- _ => rename Hf into HF3' end.
+      pose proof (Forall2_length _ _ _ Heq) as Hlenττ'.
+      destruct (struct_fields_ser_inv _ _ _ _ _ HF3' Hlen) as (ρs2 & -> & _ & HF3'').
+      pose proof (Forall3_length_lm _ _ _ _ HF3) as Hl1.
+      pose proof (Forall3_length_lr _ _ _ _ HF3) as Hl2.
+      pose proof (Forall3_length_lm _ _ _ _ HF3'') as Hl3.
+      pose proof (Forall3_length_lr _ _ _ _ HF3'') as Hl4.
+      apply eval_kind_ser_prod_struct; try congruence.
+      by eapply eval_kind_pairs_of_kinds.
+    - intros κ_ser κ_prod κ_struct κs_ser τs τs' Hlen Heq IH F κ κ' Hκ Hκ'.
+      inversion Hκ; subst.
+      match goal with
+        Hf : Forall3 _ (zip_with SerT _ _) _ _ |- _ => rename Hf into HF3' end.
+      inversion Hκ'; subst.
+      match goal with Hp : has_kind _ (ProdT _ _) _ |- _ => rename Hp into Hprod end.
+      inversion Hprod; subst.
+      match goal with Hf : Forall3 _ τs' _ _ |- _ => rename Hf into HF3 end.
+      pose proof (Forall2_length _ _ _ Heq) as Hlenττ'.
+      destruct (struct_fields_ser_inv _ _ _ _ _ HF3' Hlen) as (ρs2 & -> & _ & HF3'').
+      pose proof (Forall3_length_lm _ _ _ _ HF3) as Hl1.
+      pose proof (Forall3_length_lr _ _ _ _ HF3) as Hl2.
+      pose proof (Forall3_length_lm _ _ _ _ HF3'') as Hl3.
+      pose proof (Forall3_length_lr _ _ _ _ HF3'') as Hl4.
+      symmetry.
+      apply eval_kind_ser_prod_struct; try congruence.
+      eapply eval_kind_pairs_of_kinds; [|exact HF3|exact HF3''].
+      apply Forall2_flip in IH.
+      eapply Forall2_impl; first exact IH.
+      intros ta tb HP Fx κa κb Hka Hkb.
+      symmetry.
+      by eapply HP.
+  Qed.
+
+End pure_kinds.
+
+Section type_eq_sem.
+
+  Context `{!logrel_na_invs Σ}.
+  Context `{!wasmG Σ}.
+  Context `{!richwasmG Σ}.
+
+  Variable rti : rt_invariant Σ.
+  Variable sr : store_runtime.
+
+  Lemma big_sepL2_svr_transport {A : Type} (Ts Ts' : list (semantic_type (Σ:=Σ)))
+      (xs : list A) (f : semantic_type -> A -> iProp Σ) :
+    Forall2 (fun T T' => forall x, f T x ⊣⊢ f T' x) Ts Ts' ->
+    ([∗ list] T;x ∈ Ts;xs, f T x) ⊣⊢ ([∗ list] T;x ∈ Ts';xs, f T x).
+  Proof.
+    intros HF2.
+    revert xs.
+    induction HF2 as [|T T' Ts Ts' HTT' HF2 IH]; intros xs; first done.
+    destruct xs as [|x xs].
+    - iSplit; iIntros "H"; iDestruct (big_sepL2_length with "H") as %Hlen; done.
+    - rewrite !big_sepL2_cons HTT' IH.
+      done.
+  Qed.
+
+  Lemma type_interp_type_eq :
+    forall τ τ',
+      type_eq τ τ' ->
+      forall F κ κ' se sv,
+        has_kind F τ κ ->
+        has_kind F τ' κ' ->
+        sem_env_interp F se ->
+        type_interp rti sr τ se sv ⊣⊢ type_interp rti sr τ' se sv.
+  Proof.
+    apply (type_eq_ind'
+             (fun τ τ' =>
+                forall F κ κ' se sv,
+                  has_kind F τ κ ->
+                  has_kind F τ' κ' ->
+                  sem_env_interp F se ->
+                  type_interp rti sr τ se sv ⊣⊢ type_interp rti sr τ' se sv)).
+    - done.
+    - intros κ0 τs τs' Heq IH F κ κ' se sv Hκ Hκ' Hse.
+      admit.
+    - intros κ0 τs τs' Heq IH F κ κ' se sv Hκ Hκ' Hse.
+      admit.
+    - intros κ0 τs τs' Heq IH F κ κ' se sv Hκ Hκ' Hse.
+      admit.
+    - intros κ0 τs τs' Heq IH F κ κ' se sv Hκ Hκ' Hse.
+      admit.
+    - intros κ0 μ β τ τ' Heq IH F κ κ' se sv Hκ Hκ' Hse.
+      admit.
+    - intros κ0 τ τ' Heq IH F κ κ' se sv Hκ Hκ' Hse.
+      inversion Hκ; subst.
+      inversion Hκ'; subst.
+      match goal with Hk : has_kind F τ (VALTYPE _ _) |- _ => rename Hk into Hkτ end.
+      match goal with Hk : has_kind F τ' (VALTYPE _ _) |- _ => rename Hk into Hkτ' end.
+      rewrite !type_interp_eq.
+      iSplit.
+      + iIntros "H".
+        iDestruct "H" as (sκ) "(%Hsk & %Hsv & Hser)".
+        iExists sκ.
+        iSplit; first (iPureIntro; exact Hsk).
+        iSplit; first done.
+        iDestruct "Hser" as (os) "[%Hws Hτ]".
+        iExists os.
+        iSplit; first done.
+        by iEval (rewrite (IH F _ _ se _ Hkτ Hkτ' Hse)) in "Hτ".
+      + iIntros "H".
+        iDestruct "H" as (sκ) "(%Hsk & %Hsv & Hser)".
+        iExists sκ.
+        iSplit; first (iPureIntro; exact Hsk).
+        iSplit; first done.
+        iDestruct "Hser" as (os) "[%Hws Hτ]".
+        iExists os.
+        iSplit; first done.
+        by iEval (rewrite -(IH F _ _ se _ Hkτ Hkτ' Hse)) in "Hτ".
+    - intros κ0 τ τ' Heq IH F κ κ' se sv Hκ Hκ' Hse.
+      admit.
+    - intros κ0 τ τ' Heq IH F κ κ' se sv Hκ Hκ' Hse.
+      admit.
+    - intros κ0 τ τ' Heq IH F κ κ' se sv Hκ Hκ' Hse.
+      admit.
+    - intros κ0 τ τ' Heq IH F κ κ' se sv Hκ Hκ' Hse.
+      admit.
+    - intros κ0 κτ τ τ' Heq IH F κ κ' se sv Hκ Hκ' Hse.
+      admit.
+    - intros κ_ser κ_prod κ_struct κs_ser τs τs' Hlen Heq IH F κ κ' se sv Hκ Hκ' Hse.
+      admit.
+    - intros κ_ser κ_prod κ_struct κs_ser τs τs' Hlen Heq IH F κ κ' se sv Hκ Hκ' Hse.
+      admit.
+  Admitted.
+
+End type_eq_sem.
